SlowTest/SmallestMissingNumber-functional.dfy
@@ -13,11 +13,14 @@ method Main() {
   assert s == 0;
   print s, " ";  // 0
   var a := Cons(2, Cons(0, Nil));
-  print SmallestMissingNumber(a), " ";  // 1
+  assert SmallestMissingNumber(a) == 1;
+  // print SmallestMissingNumber(a), " ";  // 1
   a := Cons(3, Cons(1, a));
-  print SmallestMissingNumber(a), " ";  // 4
+  assert SmallestMissingNumber(a) == 4;
+  // print SmallestMissingNumber(a), " ";  // 4
   a := Cons(7, Cons(4, Cons(6, a)));
-  print SmallestMissingNumber(a), "\n";  // 5
+  assert SmallestMissingNumber(a) == 5;
+  // print SmallestMissingNumber(a), "\n";  // 5
 }
 
 // standard definitions
@@ -216,74 +219,76 @@ function IntRange(lo: nat, len: nat): set<nat>
   S
 }
 
-// ----- Proofs of alternative versions
+// Timeout proofs
 
-lemma SMN'_Correct(xs: List<nat>, n: nat, len: nat)
-  requires NoDuplicates(xs)
-  requires forall x :: x in Elements(xs) ==> n <= x
-  requires len == Length(xs)
-  ensures var s := SMN'(xs, n, len);
-    n <= s <= n + len &&
-    s !in Elements(xs) &&
-    forall x :: n <= x < s ==> x in Elements(xs)
-  decreases len
-{
-  if xs == Nil {
-  } else {
-    var half := (len + 1) / 2;
-    var (L, R) := Split(xs, n + half);
-    Split_Correct(xs, n + half);
-    var llen := Length(L);
-    Elements_Property(L);  // use the NoDuplicates property
-    var bound := IntRange(n, half);
-    Cardinality(Elements(L), bound);
-    if llen < half {
-      SMN'_Correct(L, n, llen);
-    } else {
-      var s := SMN'(R, n + llen, len - llen);
-      SMN'_Correct(R, n + llen, len - llen);
-      forall x | n <= x < s
-        ensures x in Elements(xs)
-      {
-        if x < n + llen {
-          SetEquality(Elements(L), bound);
-        }
-      }
-    }
-  }
-}
+// // ----- Proofs of alternative versions
 
-lemma SMN''_Correct(xs: List<nat>, n: nat, len: nat)
-  requires NoDuplicates(xs)
-  requires forall x :: x in Elements(xs) ==> n <= x
-  requires len == Length(xs)
-  ensures var s := SMN''(xs, n, len);
-    n <= s <= n + len &&
-    s !in Elements(xs) &&
-    forall x :: n <= x < s ==> x in Elements(xs)
-  decreases len
-{
-  if xs == Nil {
-  } else {
-    var half := len / 2 + 1;
-    var (L, R) := Split(xs, n + half);
-    Split_Correct(xs, n + half);
-    var llen := Length(L);
-    Elements_Property(L);  // use the NoDuplicates property
-    var bound := IntRange(n, half);
-    Cardinality(Elements(L), bound);
-    if llen < half {
-      SMN''_Correct(L, n, llen);
-    } else {
-      var s := SMN''(R, n + llen, len - llen);
-      SMN''_Correct(R, n + llen, len - llen);
-      forall x | n <= x < s
-        ensures x in Elements(xs)
-      {
-        if x < n + llen {
-          SetEquality(Elements(L), bound);
-        }
-      }
-    }
-  }
-}
+// lemma SMN'_Correct(xs: List<nat>, n: nat, len: nat)
+//   requires NoDuplicates(xs)
+//   requires forall x :: x in Elements(xs) ==> n <= x
+//   requires len == Length(xs)
+//   ensures var s := SMN'(xs, n, len);
+//     n <= s <= n + len &&
+//     s !in Elements(xs) &&
+//     forall x :: n <= x < s ==> x in Elements(xs)
+//   decreases len
+// {
+//   if xs == Nil {
+//   } else {
+//     var half := (len + 1) / 2;
+//     var (L, R) := Split(xs, n + half);
+//     Split_Correct(xs, n + half);
+//     var llen := Length(L);
+//     Elements_Property(L);  // use the NoDuplicates property
+//     var bound := IntRange(n, half);
+//     Cardinality(Elements(L), bound);
+//     if llen < half {
+//       SMN'_Correct(L, n, llen);
+//     } else {
+//       var s := SMN'(R, n + llen, len - llen);
+//       SMN'_Correct(R, n + llen, len - llen);
+//       forall x | n <= x < s
+//         ensures x in Elements(xs)
+//       {
+//         if x < n + llen {
+//           SetEquality(Elements(L), bound);
+//         }
+//       }
+//     }
+//   }
+// }
+
+// lemma SMN''_Correct(xs: List<nat>, n: nat, len: nat)
+//   requires NoDuplicates(xs)
+//   requires forall x :: x in Elements(xs) ==> n <= x
+//   requires len == Length(xs)
+//   ensures var s := SMN''(xs, n, len);
+//     n <= s <= n + len &&
+//     s !in Elements(xs) &&
+//     forall x :: n <= x < s ==> x in Elements(xs)
+//   decreases len
+// {
+//   if xs == Nil {
+//   } else {
+//     var half := len / 2 + 1;
+//     var (L, R) := Split(xs, n + half);
+//     Split_Correct(xs, n + half);
+//     var llen := Length(L);
+//     Elements_Property(L);  // use the NoDuplicates property
+//     var bound := IntRange(n, half);
+//     Cardinality(Elements(L), bound);
+//     if llen < half {
+//       SMN''_Correct(L, n, llen);
+//     } else {
+//       var s := SMN''(R, n + llen, len - llen);
+//       SMN''_Correct(R, n + llen, len - llen);
+//       forall x | n <= x < s
+//         ensures x in Elements(xs)
+//       {
+//         if x < n + llen {
+//           SetEquality(Elements(L), bound);
+//         }
+//       }
+//     }
+//   }
+// }
